\documentclass{article}
\usepackage[utf8]{inputenc}
\usepackage{listings}
\usepackage{multimedia} % to embed movies in the PDF file
\usepackage{graphicx}
\usepackage{comment}
\usepackage[english]{babel}
\usepackage{amsmath}
\usepackage{amsfonts}
\usepackage{subfigure}
\usepackage{wrapfig}
\usepackage{multirow}
\usepackage{verbatim}
\include{latex-defs}


\title{AMATH 568 Homework 2}
\author{Cade Ballew \#2120804}
\date{January 19, 2022}

\begin{document}
	
\maketitle
	
\section{Problem 1}
To show that, for each fixed $\ell\geq0$, the integral
\begin{align*}
	H(t) = \int_0^\infty e^{-x^2 - 2 t x} (tx)^\ell dx, \quad t \geq 0,
\end{align*}
is $\OO(1)$ for $t \in [0,\infty)$, first consider some special cases. If $t=0$, then $H(t)=0,$ so $|H(t)|\leq K$ for any $K>0$. Thus, going forward we only consider $t \in (0,\infty)$.\\
Now, consider the case where $\ell=0$. Then, 
\begin{align*}
|H(t)|=\int_0^\infty e^{-x^2 - 2t x} dx\leq\int_0^\infty e^{-x^2} dx=\frac{\sqrt{\pi}}{2},
\end{align*}
so if we take $K=\frac{\sqrt{\pi}}{2}$, we have that $|H(t)|<K*1$ for all $t \in [0,\infty)$, meaning that $H(t)$ is $\OO(1)$.\\
Now, consider $\ell>0$. Then, using the change of variables $u=2tx$,
\begin{align*}
	|H(t)| = \int_0^\infty e^{-x^2 - 2 t x} (tx)^\ell dx=\int_0^\infty e^{-\left(\frac{u}{2t}\right)^2 - u} \left(\frac{u}{2}\right)^\ell \frac{du}{2t}\leq\frac{1}{2^{\ell+1}}\int_0^\infty e^{-u}u^{\ell-1}\frac{u}{t}e^{-\left(\frac{u}{2t}\right)^2}du.
\end{align*}
Now, because we consider $t\neq0$, let $v=\frac{u}{t}$. Then,
\[
\frac{u}{t}e^{-\left(\frac{u}{2t}\right)^2}=ve^{-v^2/4}\leq\sqrt{2}e^{-1/2}=\sqrt{\frac{2}{e}}<1,
\] 
because $ve^{-v^2/4}$ is maximized at $v=\sqrt{2}$ by elementary calculus. Thus, 
\[
|H(t)|<\frac{1}{2^{\ell+1}}\int_0^\infty e^{-u}u^{\ell-1}=\frac{\Gamma(\ell)}{2^{\ell+1}}.
\]
This is constant with respect to $t$, so we simply take $K=\frac{\Gamma(\ell)}{2^{\ell+1}}$, and then $|H(t)|<K*1$ for all $t \in [0,\infty)$, meaning that $H(t)$ is $\OO(1)$.

\section{Problem 2}
We wish to apply Watson's lemma to derive an asymptotic expansion of
\begin{align*}
	F(\lambda)  = \int_0^\infty e^{-\lambda t} \frac{\sin t}{t^{3/2}} d t, \quad \lambda > 0, \quad \lambda \to \infty
\end{align*}
by taking $\phi(t)=\frac{\sin t}{t^{3/2}}$ and $g(t)=\frac{\sin t}{t}$ so that $\phi(t)=t^\sigma g(t)$ where $\sigma=-1/2>-1$. To do this, we need to show that $\phi(t)$ is absolutely integrable on $[0,\infty)$ and that $g(t)$ is infinitely differentiable in a neighborhood of $t=0$. To see that $\phi(t)$ is absolutely integrable, write 
\[
\int_0^\infty|\phi(t)|dt=\underbrace{\int_0^1\left|\frac{\sin t}{t^{3/2}}\right|dt}_{I_1}+\underbrace{\int_1^\infty\left|\frac{\sin t}{t^{3/2}}\right|dt}_{I_2}. 
\]
Using the fact that $|\sin(t)|=\sin(t)\leq t$ on $[0,1]$, 
\[
I_1\leq\int_0^1\frac{t}{t^{3/2}}dt=\int_0^1\frac{dt}{\sqrt{t}}=2.
\]
Using the fact that $|\sin{t}|\leq1$,
\[
I_2\leq\int_1^\infty\frac{dt}{t^{3/2}}=2.
\]
Thus, 
\[
\int_0^\infty|\phi(t)|dt=I_1+I_2\leq4<\infty.
\]
To see that $g(t)$ is infinitely differentiable around $t=0$, we use the Taylor series centered at $t=0$ for the sine function to write
\[
g(t)=\frac{1}{t}\sum_{j=0}^\infty(-1)^j\frac{t^{2j+1}}{(2j+1)!}=\sum_{j=0}^\infty(-1)^j\frac{t^{2j}}{(2j+1)!}=1-\frac{t^2}{3!}+\frac{t^4}{5!}-\ldots.
\]
Since this Taylor series for $\sin(t)$ holds for all $t\in\real$ and this expression for $g(t)$ is a polynomial, $g(t)$ is clearly infinitely differentiable around $t=0$. Furthermore, we can compute $g^{(j)}(0)$ by noting that it is precisely the constant term of the series for $g^{(j)}(t)$. This will be zero for odd $j$ since our series contains only even powers of $t$. Thus, we can write
\[
g^{(2j)}(0)=(-1)^j(2j)!\frac{1}{(2j+1)!}=\frac{(-1)^j}{2j+1}.
\]
With this in hand, we apply Watson's lemma and use our above expression to conclude that 
\begin{align*}
F(\lambda)\sim\sum_{n=0}^{\infty}\frac{g^{(n)}(0)\Gamma(\sigma+n+1)}{n!\lambda^{\sigma+n+1}}=\sum_{j=0}^{\infty}\frac{(-1)^j}{2j+1}\frac{\Gamma(2j+1/2)}{(2j)!\lambda^{2j+1/2}}=\sum_{j=0}^{\infty}\frac{(-1)^j\Gamma(2j+1/2)}{(2j+1)!\lambda^{2j+1/2}},
\end{align*}
as $\lambda\to\infty$ with $\lambda>0$ where we have reindexed $n\to2j$.
	
\section{Problem 3}
To derive an asymptotic expansion of \begin{align*}
	u(x,t) = \frac{1}{2 \pi} \int_{-\infty}^\infty e^{i k x - k^2 t} \hat f(k) d k, \quad \hat f(k) = \int_{-\infty}^\infty e^{-i k x} f(x) d x
\end{align*}
for fixed $x$, let $\phi(k)=e^{ikx}\hat{f}(k)$, $a=-\infty$, and $b=\infty$ and consider the generalization of Watson's lemma on page 6 of part 2 of the course notes where $f$ and $\hat f$ are assumed to decay rapidly enough so that $\phi(k)$ is absolutely integrable on $(-\infty,\infty)$ and $\phi(k)$ has an infinite number of continuous derivatives in a neighborhood of $k=0$. Then, the result on page 8 of part 2 of the notes gives that 
\[
u(x,t)\sim\frac{1}{2\pi}\sqrt{\frac{\pi}{t}}\sum_{j=0}^\infty\frac{\phi^{(2j)}(0)}{t^j}\frac{1}{2^{2j}j!}
\]
as $t\to\infty$, $t>0$. Now, we compute derivatives of $\phi(k)$. By the product rule, 
\begin{align*}
\phi'(k)&=ixe^{ikx}\int_{-\infty}^\infty e^{-ikx}f(x)dx+e^{ikx}\int_{-\infty}^\infty \frac{d}{dk}(e^{-ikx}f(x))dx\\&=
ixe^{ikx}\int_{-\infty}^\infty e^{-ikx}f(x)dx-e^{ikx}\int_{-\infty}^\infty ixe^{-ikx}f(x)dx
\end{align*}
Again, by the product rule,
\begin{align*}
\phi''(k)&=(ix)^2e^{ikx}\int_{-\infty}^\infty e^{-ikx}f(x)dx-ixe^{ikx}\int_{-\infty}^\infty ix e^{-ikx}f(x)dx\\&-ixe^{ikx}\int_{-\infty}^\infty ix e^{-ikx}f(x)dx+e^{ikx}\int_{-\infty}^\infty (ix)^2e^{-ikx}f(x)dx\\&=
(ix)^2e^{ikx}\int_{-\infty}^\infty e^{-ikx}f(x)dx-2ixe^{ikx}\int_{-\infty}^\infty ix e^{-ikx}f(x)dx+e^{ikx}\int_{-\infty}^\infty (ix)^2e^{-ikx}f(x)dx.
\end{align*}
Thus, we can compute
\[
\phi(0)=\hat{f}(0)=\int_{-\infty}^\infty f(x)dx
\]
and
\begin{align*}
\phi''(0)&=(ix)^2\int_{-\infty}^\infty f(x)dx-2ix\int_{-\infty}^\infty ix f(x)dx+\int_{-\infty}^\infty (ix)^2f(x)dx\\&=
-x^2\int_{-\infty}^\infty f(x)dx+2x\int_{-\infty}^\infty xf(x)dx-\int_{-\infty}^\infty x^2f(x)dx.
\end{align*}
Now, we can simply plug in $j=0,1$ to find the first two nonzero terms of our expansion. Namely, the first term is given by
\[
\frac{1}{2\pi}\sqrt{\frac{\pi}{t}}\phi(0)=\frac{1}{2\pi}\sqrt{\frac{\pi}{t}}\int_{-\infty}^\infty f(x)dx
\]
and the second term is given by
\begin{align*}
\frac{1}{2\pi}\sqrt{\frac{\pi}{t}}\frac{\phi''(0)}{t}\frac{1}{2^{2}1!}=
\frac{1}{2\pi}\sqrt{\frac{\pi}{t}}\frac{1}{4t}\left(-x^2\int_{-\infty}^\infty f(x)dx+2x\int_{-\infty}^\infty xf(x)dx-\int_{-\infty}^\infty x^2f(x)dx\right).
\end{align*}
	
\section{Problem 4}
To compute the asymptotic expansion of
\begin{align*}
	u(x,t) = \frac{1}{2 \pi} \int_{-\infty}^\infty e^{i k x - k^4 t} \hat f(k) d k, \quad \hat f(k) = \int_{-\infty}^\infty e^{-i k x} f(x) d x,
\end{align*}
we derive an additional generalization of Watson's lemma based on the generalization used in problem 3. Namely, we consider 
\[
F(\lambda)=\int_a^b e^{-\lambda t^4}\phi(t)dt
\]
where $a<0<b$, $\lambda>0$, and $\phi(t)$ is absolutely integrable and has an infinite number of continuous derivatives in a neighborhood of $t=0$.\\
Steps 1 and 2 of our derivation are essentially the same as their counterparts on page 7 of part 2 of the course notes. Namely, to localize, fix $\epsilon>0$. Then,
\[
\int_a^b e^{-\lambda t^4}\phi(t)dt=\int_{-\epsilon}^\epsilon e^{-\lambda t^4}\phi(t)dt+\OO(\lambda^{-N})
\]
as $\lambda\to\infty$, $\lambda>0$ for all $N>0$ since the absolute integrability of $\phi(t)$ allows us to bound the integrals on the remaining domain by a constant times $e^{-\lambda\epsilon^4}$.\\
Using the remainder estimate, 
\[
\int_{-\epsilon}^\epsilon e^{-\lambda t^4}\phi(t)dt=\int_{-\epsilon}^\epsilon e^{-\lambda t^4}\left(\sum_{j=0}^N\phi^{(j)}(0)\frac{t^j}{j!}-r_N(t)\right)dt
\]
where $r_N(t)=\OO(t^{N+1})$ as $t\to0$. \\
To find large $\lambda$ limits, we use the substitution $s=\sqrt[4]{\lambda}t$ to get
\[
\int_{-\epsilon}^\epsilon e^{-\lambda t^4}t^\ell dt=\int_{-\sqrt[4]{\lambda}\epsilon}^{\sqrt[4]{\lambda}\epsilon} e^{-s^4}\left(\frac{s}{\sqrt[4]{\lambda}}\right)^\ell\frac{ds}{\sqrt[4]{\lambda}}=\frac{1}{\lambda^{\ell/4+1/4}}\int_{-\sqrt[4]{\lambda}\epsilon}^{\sqrt[4]{\lambda}\epsilon} e^{-s^4}s^\ell ds=\OO(\lambda^{-\ell/4-1/4}).
\]
To see this, first note that if $\ell$ is odd, 
\[
\int_{-\sqrt[4]{\lambda}\epsilon}^{\sqrt[4]{\lambda}\epsilon} e^{-s^4}s^\ell ds=0
\] 
by the symmetry of $e^{-s^4}$. If $\ell$ is even, the same symmetry gives that 
\[
\int_{-\sqrt[4]{\lambda}\epsilon}^{\sqrt[4]{\lambda}\epsilon} e^{-s^4}s^\ell ds=\int_{-\infty}^{\infty} e^{-s^4}s^\ell ds-2\int_{\sqrt[4]{\lambda}\epsilon}^{\infty} e^{-s^4}s^\ell ds.
\]
Then, using the change of variables $s=\sqrt[4]{\lambda}\epsilon+x$,
\begin{align*}
\int_{\sqrt[4]{\lambda}\epsilon}^{\infty} e^{-s^4}s^\ell ds&=\int_0^\infty e^{-\lambda\epsilon^4-4\sqrt[4]{\lambda^3}\epsilon^3x-6\sqrt{\lambda}\epsilon^2x^2-4\sqrt[4]{\lambda}\epsilon x^3-x^4}(\sqrt[4]{\lambda}\epsilon+x)^\ell dx\\&\leq
e^{-\lambda\epsilon^4}\int_0^\infty e^{-x^4/2}(\underbrace{\sqrt[4]{\lambda}\epsilon e^{-\frac{x^4}{2\ell}}}_{\leq \sqrt[4]{\lambda}\epsilon}+\underbrace{xe^{-\frac{x^4}{2\ell}}}_{\leq C})^\ell dx\\&\leq e^{-\lambda\epsilon^4}(\sqrt[4]{\lambda}\epsilon+C)^\ell\int_0^\infty e^{-x^4/2}dx=\OO(\lambda^{-N})
\end{align*}
for all $N>0$ as $\lambda\to\infty$ when $\lambda>0$. Additionally, when $\ell$ is even, using the substitution $t=s^4$,
\[
\int_{-\infty}^{\infty} e^{-s^4}s^\ell ds=2\int_{0}^{\infty} e^{-s^4}s^\ell ds=2\int_{0}^{\infty} e^{-t}t^{\ell/4}\frac{dt}{4t^{3/4}}=\frac{1}{2}\Gamma(\frac{\ell}{4}+\frac{1}{4}).
\]
Now, we can assemble everything to conclude that 
\[
F(\lambda)\sim\sum_{j=0}^\infty\frac{\phi^{(2j)}(0)}{(2j)!\lambda^{j/2+1/4}}\frac{\Gamma(j/2+1/4)}{2}
\]
where we have reindexed $\ell\to2j$ to account for only the even terms being nonzero.\\
Now, taking $\phi(k)=e^{ikx}\hat{f}(k)$, $a=-\infty$, and $b=\infty$ as in problem 3 and again assuming that $f$ and $\hat{f}$ decay rapidly so that $\phi(k)$ is absolutely integrable on $(-\infty,\infty)$ and $\phi(k)$ has an infinite number of continuous derivatives in a neighborhood of $k=0$, we have that 
\[
u(x,t)\sim\frac{1}{2\pi} \sum_{j=0}^\infty\frac{\phi^{(2j)}(0)}{(2j)!t^{j/2+1/4}}\frac{\Gamma(j/2+1/4)}{2}
\]
as $t\to\infty$, $t>0$. Since we have computed the required derivatives in problem 3, we plug in $j=0,1$ and conclude that the first term is given by 
\[
\frac{1}{2\pi}\frac{\Gamma(1/4)}{2t^{1/4}}\int_{-\infty}^\infty f(x)dx
\]
and the second term is given by
\[
\frac{1}{2\pi}\frac{\Gamma(3/4)}{4t^{3/4}}\left(-x^2\int_{-\infty}^\infty f(x)dx+2x\int_{-\infty}^\infty xf(x)dx-\int_{-\infty}^\infty x^2f(x)dx\right).
\]
This expansion differs from that in problem 3 in that its leading term has $t$ raised to $-1/4$ instead of $-1/2$. Additionally, each successive term has the power of its $t$ term decreased by $1/2$ instead of $1$, meaning that it will take more terms to get an approximation of a similar order if we are considering large $t$. 
	
\end{document}
