\documentclass{article}
\usepackage[utf8]{inputenc}
\usepackage{listings}
\usepackage{multimedia} % to embed movies in the PDF file
\usepackage{graphicx}
\usepackage{comment}
\usepackage[english]{babel}
\usepackage{amsmath}
\usepackage{amsfonts}
\usepackage{wrapfig}
\usepackage{multirow}
\usepackage{verbatim}
\usepackage{float}
\usepackage{cancel}
\usepackage{caption}
\usepackage{subcaption}
\usepackage{cancel}
\include{latex-defs}


\title{AMATH 515 Homework 4}
\author{Cade Ballew}
\date{March 16, 2022}

\begin{document}
	
\maketitle
	
\section{Problem 1}
Let $\alpha\in\real$. Then,
\begin{align*}
&\|\alpha x + (1-\alpha) y\|^2 + \alpha(1-\alpha) \|x-y\|^2\\&=
\|\alpha x\|^2+2\ip{\alpha x}{(1-\alpha) y}+\|(1-\alpha) y\|^2+ \alpha(1-\alpha)\left(\|x\|^2-2\ip{x}{y}+\|y\|^2\right)\\&=
\alpha^2\|x\|^2+\cancel{2\alpha(1-\alpha)\ip{x}{ y}}+(1-\alpha)^2\| y\|^2+ \alpha(1-\alpha)\|x\|^2-\cancel{2\alpha(1-\alpha)\ip{x}{y}}+\alpha(1-\alpha)\|y\|^2\\&=
\alpha(\alpha+(1-\alpha))\|x\|^2+(1-\alpha)((1-\alpha)+\alpha)\|y\|^2=\alpha \|x\|^2 + (1-\alpha) \|y\|^2.
\end{align*}

\section{Problem 2}
Let 
\[
T_\lambda = (1-\lambda)I + \lambda T
\]
where $T$ is nonexpansive. 
\subsection{Part a}
To see that $T_\lambda$ and $T$ have the same fixed points, consider an $x$ such that $x=Tx$ (a fixed point of $T$). Then,
\[
T_\lambda x=((1-\lambda)I + \lambda T)x=(1-\lambda)x+\lambda Tx=(1-\lambda)x+\lambda x=x,
\]
so $x$ is a fixed point of $T_\lambda$. If $x$ is instead a fixed point of $T_\lambda$, then $T_\lambda x=x$, so
\[
x=T_\lambda x=((1-\lambda)I + \lambda T)x=(1-\lambda)x+\lambda Tx.
\]
Then,
\[
\lambda Tx=x-(1-\lambda)x=\lambda x,
\]
so $Tx=x$, meaning that $x$ is also a fixed point of $T$. Thus, $T$ and $T_\lambda$ have the same fixed points.  

\subsection{Part b}
Let $\overline z$ be a fixed point of $T$. Then, $\overline z=T\overline z$, so
\begin{align*}
\|T_\lambda z - \overline z\|^2=\|(1-\lambda)z + \lambda Tz - \lambda\overline z -(1-\lambda)\overline z\|^2=\|\lambda (Tz-T\Bar{z})+(1-\lambda)(z-\Bar{z})\|^2.
\end{align*}
Now, we apply problem 1 and use the fact that $T$ is nonexpansive to get that 
\begin{align*}
\|T_\lambda z - \overline z\|^2&=\lambda\|Tz-T\Bar{z}\|^2+(1-\lambda)\|z-\Bar{z}\|^2-\lambda(1-\lambda)\|(Tz-T\Bar{z})-(z-\Bar{z})\|^2\\&\leq
\lambda\|z-\Bar{z}\|^2+(1-\lambda)\|z-\Bar{z}\|^2-\lambda(1-\lambda)\|Tz-\underbrace{T\Bar{z}}_{=\Bar{z}}-z+\Bar{z}\|^2\\&=
\|z-\Bar{z}\|^2-\lambda(1-\lambda)\|Tz-z\|^2=\|z-\Bar{z}\|^2-\lambda(1-\lambda)\|z-Tz\|^2.
\end{align*}

\section{Problem 3}
\subsection{Part a}
Let $T$ be a firmly nonexpansive operator. Then, 
\[
\|Tx - Ty\|^2 + \|(I-T) x - (I-T)y\|^2 \leq \|x-y\|^2. 
\]
From this, 
\begin{align*}
\text{LHS}&=\|Tx - Ty\|^2+\|(x-y)-(Tx-Ty)\|^2\\&=
\|Tx - Ty\|^2+\|x-y\|^2-2\ip{x-y}{Tx-Ty}+\|Tx-Ty\|^2\\&=
2\|Tx - Ty\|^2+\|x-y\|^2-2\ip{x-y}{Tx-Ty}.
\end{align*}
Thus, by definition, $T$ is firmly nonexpansive iff
\[
2\|Tx - Ty\|^2+\|x-y\|^2-2\ip{x-y}{Tx-Ty}\leq\|x-y\|^2. 
\]
Of course, we can just move terms around to see that this is true iff, 
\[
\langle x-y, Tx - Ty \rangle \geq \|Tx - Ty\|^2,
\]
so $T$ is firmly nonexpansive iff this holds.

\subsection{Part b}
Using the result of part a, we can write the norm as an inner product to get that $T$ is firmly nonexpansive iff
\[
\langle x-y, Tx - Ty \rangle-\ip{Tx - Ty}{Tx - Ty}\geq0.
\]
Now, note that
\begin{align*}
&\langle x-y, Tx - Ty \rangle-\ip{Tx - Ty}{Tx - Ty}\\&=
\ip{(x-y)-(Tx-Ty)}{Tx - Ty}=\ip{(I-T)x-(I-T)y}{Tx-Ty}.
\end{align*}
Thus, $T$ is firmly nonexpansive iff
\[
\langle Tx - Ty, (I-T)x - (I-T)y \rangle \geq 0.
\]

\subsection{Part c}
Now, suppose that $S = 2T - I$. Let 
\[
\mu = \|Tx - Ty\|^2 + \|(I-T)x - (I-T)y\|^2 - \|x-y\|^2
\]
and let 
\[
\nu = \|Sx - Sy\|^2 - \|x-y\|^2.
\]
Then, 
\begin{align*}
\nu &= \|(2T-I)x-(2T-I)y\|^2-\|x-y\|^2 \\&=
\|(T-I)x-(T-I)y+(Tx-Ty)\|^2+\|x-y\|^2-2\|x-y\|^2\\&=
\|(T-I)x-(T-I)y+(Tx-Ty)\|^2\\&+\|(T-I)x-(T-I)y-(Tx-Ty)\|^2-2\|x-y\|^2,
\end{align*}
so
\begin{align*}
\frac{1}{4}\nu&=\|\frac{1}{2}((T-I)x-(T-I)y)+\frac{1}{2}(Tx-Ty)\|^2\\&+\frac{1}{4}\|(T-I)x-(T-I)y-(Tx-Ty)\|^2-\frac{1}{2}\|x-y\|^2.
\end{align*}
Applying problem 1 with $\alpha=\frac{1}{2}$ to the first two terms, we get that 
\begin{align*}
    \frac{1}{4}\nu&=\frac{1}{2}\|(T-I)x-(T-I)y\|^2+\frac{1}{2}\|Tx-Ty\|^2-\frac{1}{2}\|x-y\|^2,
\end{align*}
so
\begin{align*}
\nu&=2\|(T-I)x-(T-I)y\|^2+2\|Tx-Ty\|^2-2\|x-y\|^2=2\mu.
\end{align*}
We know from the definition that $T$ is firmly nonexpansive iff $\mu\leq0$ which we now know is true iff $\nu\leq0$. Of course, this is true iff $S$ is nonexpansive.

\end{document}